infra/GetSucc.v
@@ -1,0 +1,14 @@
+
+Require Import ListOrder.
+
+Fixpoint get_succ (A : eqType) (a e : A) (l : list A)
+  := match l with
+     | nil => e
+     | b :: l => if decision (a = b) then e else get_succ a b l
+     end.
+
+Lemma get_succ_cons (A : eqType) (l : list A) (a b : A)
+      (Hel : a ∈ l)
+  : get_succ a b l ≻ a | b :: l.
+Proof.
+Admitted.
